modules/Mod2STS.v
@@ -28,8 +28,8 @@ Section EXEC.
 
   Definition ths_state : Type := nat * list (itree modE Any.t).
 
-  Definition handle_schE_callE (prog: callE ~> itree modE):
-    ths_state -> itree (stateE +' coreE) (ths_state + Any.t) :=
+  Definition handle_schE_callE (prog: callE ~> itree modE)
+      : ths_state -> itree (stateE +' coreE) (ths_state + Any.t) :=
     fun '(tid, ths) =>
       itr <- (base.lookup tid ths)? ;;
       match observe (itr: itree modE Any.t) with
@@ -54,11 +54,11 @@ Section EXEC.
       end.
 
   Definition interp_schE_callE (prog: callE ~> itree modE) (itr0: itree modE Any.t)
-    : itree (stateE +' coreE) Any.t
-    :=
+      : itree (stateE +' coreE) Any.t :=
     ITree.iter (handle_schE_callE prog) (0, [itr0]).
 
-  Definition interp_modE (prog: callE ~> itree modE) (itr0: itree modE Any.t) (st0: Any.t): itree coreE _ :=
+  Definition interp_modE (prog: callE ~> itree modE) (itr0: itree modE Any.t) (st0: Any.t)
+      : itree coreE _ :=
     interp_stateE Any.t (interp_schE_callE prog itr0) st0.
 
 End EXEC.
@@ -76,28 +76,18 @@ Section SEMANTICS.
     end.
 
   Inductive step: state -> option event -> state -> Prop :=
-  | step_tau
-      itr
-    :
+  | step_tau itr :
       step (Tau itr) None itr
-  | step_choose
-      X k (x: X)
-    :
+  | step_choose X k (x : X) :
       step (Vis (subevent _ (Choose X)) k) None (k x)
-  | step_take
-      X k (x: X)
-    :
+  | step_take X k (x : X) :
       step (Vis (subevent _ (Take X)) k) None (k x)
-  | step_io
-      fn I O (args: I) (rv: O) k
-    :
+  | step_io fn I O (args: I) (rv: O) k :
       step (Vis (subevent _ (IO fn args)) k) (Some (event_io fn args rv)) (k rv).
 
   Lemma step_trigger_choose_iff X k itr e
-        (STEP: step (trigger (Choose X) >>= k) e itr)
-    :
-      exists x,
-        e = None /\ itr = k x.
+        (STEP: step (trigger (Choose X) >>= k) e itr) :
+    exists x, e = None /\ itr = k x.
   Proof.
     inv STEP.
     { eapply f_equal with (f:=observe) in H0. ss. }
@@ -109,10 +99,8 @@ Section SEMANTICS.
   Qed.
 
   Lemma step_trigger_take_iff X k itr e
-        (STEP: step (trigger (Take X) >>= k) e itr)
-    :
-      exists x,
-        e = None /\ itr = k x.
+        (STEP: step (trigger (Take X) >>= k) e itr) :
+    exists x, e = None /\ itr = k x.
   Proof.
     inv STEP.
     { eapply f_equal with (f:=observe) in H0. ss. }
@@ -124,25 +112,18 @@ Section SEMANTICS.
   Qed.
 
   Lemma step_tau_iff itr0 itr1 e
-        (STEP: step (Tau itr0) e itr1)
-    :
-      e = None /\ itr0 = itr1.
-  Proof.
-    inv STEP. et.
-  Qed.
+        (STEP: step (Tau itr0) e itr1) :
+    e = None /\ itr0 = itr1.
+  Proof. inv STEP. et. Qed.
 
   Lemma step_ret_iff rv itr e
-        (STEP: step (Ret rv) e itr)
-    :
-      False.
-  Proof.
-    inv STEP.
-  Qed.
+        (STEP: step (Ret rv) e itr) :
+    False.
+  Proof. inv STEP. Qed.
 
   Lemma step_trigger_io_iff fn I O args k e itr
-        (STEP: step (trigger (@IO I O fn args) >>= k) e itr)
-    :
-      exists rv, itr = k rv /\ e = Some (event_io fn args rv).
+        (STEP: step (trigger (@IO I O fn args) >>= k) e itr) :
+    exists rv, itr = k rv /\ e = Some (event_io fn args rv).
   Proof.
     inv STEP.
     { eapply f_equal with (f:=observe) in H0. ss. }
@@ -153,19 +134,17 @@ Section SEMANTICS.
       dependent destruction H0. ired. et. }
   Qed.
 
-  Let itree_eta E R (itr0 itr1: itree E R)
-      (OBSERVE: observe itr0 = observe itr1)
-    :
-      itr0 = itr1.
+  Local Lemma itree_eta E R (itr0 itr1: itree E R)
+      (OBSERVE: observe itr0 = observe itr1) :
+    itr0 = itr1.
   Proof.
     rewrite (itree_eta_ itr0).
     rewrite (itree_eta_ itr1).
     rewrite OBSERVE. auto.
   Qed.
 
-  Lemma step_trigger_choose X k x
-    :
-      step (trigger (Choose X) >>= k) None (k x).
+  Lemma step_trigger_choose X k x :
+    step (trigger (Choose X) >>= k) None (k x).
   Proof.
     unfold trigger. ss.
     match goal with
@@ -177,9 +156,8 @@ Section SEMANTICS.
       extensionality x0. eapply itree_eta. ss. }
   Qed.
 
-  Lemma step_trigger_take X k x
-    :
-      step (trigger (Take X) >>= k) None (k x).
+  Lemma step_trigger_take X k x :
+    step (trigger (Take X) >>= k) None (k x).
   Proof.
     unfold trigger. ss.
     match goal with
@@ -191,9 +169,8 @@ Section SEMANTICS.
       extensionality x0. eapply itree_eta. ss. }
   Qed.
 
-  Lemma step_trigger_io I O fn (args: I) k (rv: O)
-    :
-      step (trigger (IO fn args) >>= k) (Some (event_io fn args rv)) (k rv).
+  Lemma step_trigger_io I O fn (args: I) k (rv: O) :
+    step (trigger (IO fn args) >>= k) (Some (event_io fn args rv)) (k rv).
   Proof.
     unfold trigger. ss.
     match goal with
@@ -204,7 +181,6 @@ Section SEMANTICS.
     { eapply itree_eta. ss. cbv. f_equal.
       extensionality x0. eapply itree_eta. ss. }
   Qed.
-
 
   Program Definition compile_itree: itree coreE Any.t -> semantics :=
     fun itr =>
