modules/Mod.v
@@ -12,17 +12,18 @@ Require Import Events.
 Set Implicit Arguments.
 
 Section ADD.
+
   Definition RUN : Type := forall V, (Any.t -> Any.t * V) -> (Any.t -> Any.t * V).
 
   Definition run_l: RUN := 
-    fun V run st =>
+    fun _ run st =>
       match Any.split st with
       | Some (a, b) => let (a', v) := run a in (Any.pair a' b, v)
       | None => run tt↑
       end.
 
   Definition run_r: RUN := 
-    fun V run st =>
+    fun _ run st =>
       match Any.split st with
       | Some (a, b) => let (b', v) := run b in (Any.pair a b', v)
       | None => run tt↑
@@ -31,41 +32,42 @@ Section ADD.
 End ADD.
 
 Module ModSem.
-Section MODSEM.
+  Section MODSEM.
 
-  Record t: Type := mk {
-    initial_st : Any.t;
-    fnsems : alist gname (Any.t -> itree modE Any.t);
-  }.
+    Record t: Type := mk {
+      initial_st : Any.t;
+      fnsems : alist gname (Any.t -> itree modE Any.t);
+    }.
 
-  Record wf (ms: t): Prop := mk_wf {
-    wf_fnsems: List.NoDup (List.map fst ms.(fnsems));
-  }.
+    Record wf (ms: t): Prop := mk_wf {
+      wf_fnsems: List.NoDup (List.map fst ms.(fnsems));
+    }.
 
-  Definition empty: t := {|
-    initial_st := tt↑;
-    fnsems := [];
-  |}.
+    Definition empty: t := {|
+      initial_st := tt↑;
+      fnsems := [];
+    |}.
 
-  Definition init (body: itree modE Any.t) : t := {|
-    initial_st := tt↑;
-    fnsems := [("CCR_init", fun _ => body)];
-  |}.
+    Definition init (body: itree modE Any.t) : t := {|
+      initial_st := tt↑;
+      fnsems := [("CCR_init", fun _ => body)];
+    |}.
 
-  Section COMPILE.
-    Variable ms: t.
+    Section COMPILE.
+    
+      Variable ms: t.
 
-    Definition prog: callE ~> itree modE :=
-      fun _ '(Call fn args) =>
-        sem <- (alist_find fn ms.(fnsems))?;;
-        sem args.
+      Definition prog: callE ~> itree modE :=
+        fun _ '(Call fn args) =>
+          sem <- (alist_find fn ms.(fnsems))?;;
+          sem args.
 
-    Definition initial_itr : itree coreE Any.t :=
-      snd <$> interp_modE prog (prog (Call "CCR_init" ()↑)) (initial_st ms).
+      Definition initial_itr : itree coreE Any.t :=
+        snd <$> interp_modE prog (prog (Call "CCR_init" ()↑)) (initial_st ms).
 
-    Definition compile : semantics:=
-      compile_itree (initial_itr).
+      Definition compile : semantics:=
+        compile_itree (initial_itr).
 
-  End COMPILE.
-End MODSEM.
+    End COMPILE.
+  End MODSEM.
 End ModSem.
